proof/Simple_Data/Progress.v
@@ -3,98 +3,120 @@ Require Import EsJudge.
 Require Import TyJudge.
 Require Import Exp.
 Require Import Base.
+Require Import BaseList.
+
+
+Lemma step_XCon
+ :  forall  C x dc
+ ,  exps_ctx C 
+ -> (exists x', STEP x x')
+ -> (exists x', STEP (XCon dc (C x)) (XCon dc (C x'))).
+Proof.
+ intros. 
+ destruct H0 as [x'].
+ exists x'.
+ eapply (EsContext (fun xx => XCon dc (C xx))).
+ eauto. eauto.
+Qed.
+
+
 
 
 (* A well typed expression is either a well formed value, 
    or can transition to the next state.
  *)
 Theorem progress
- :  forall ds t T
- ,  TYPE ds Empty t T
- -> value t \/ (exists t', STEP t t').
+ :  forall ds x t
+ ,  TYPE ds Empty x t
+ -> value x \/ (exists x', STEP x x').
 Proof.
- intros.
- remember (@Empty ty) as tenv.
- induction H.
-
+ intros. gen t.
+ induction x using exp_mutind with 
+  (PA := fun a => a = a)
+  ; intros.
+ 
  Case "XVar".
-  subst. inverts H.
+  subst. inverts H. false.
 
  Case "XLam".
-  left. subst. eauto. 
+  left. eapply Value; eauto.
 
  Case "XApp".
-  right. 
-  specializes IHTYPE1 Heqtenv.
-  specializes IHTYPE2 Heqtenv.
-  destruct IHTYPE1.
-
-  SCase "value x1".
-   destruct IHTYPE2.
-
-   SSCase "value x2".
-    inverts H1. inverts H3.
-
-     SSSCase "x1 ~ XVar".
-      inverts H4. destruct H5. false.
-
-     SSSCase "x1 ~ XLam".
-      exists (substX 0 x2 x0).
-      apply EsLamApp.
-      inverts H2. auto.
-
-     SSSCase "x1 ~ XCon TFun".
-      inverts H. 
-
-   SSCase "x2 steps".
-    destruct H2 as [x2'].
-    exists (XApp x1 x2'). eauto.
-
-   SSCase "x1 steps".
-    destruct H1 as [x1'].
-    exists (XApp x1' x2).
-    eapply (EsContext (fun xx => XApp xx x2)); eauto.
-
+  inverts H.
+  right.
+  specializes IHx1 H4.
+  specializes IHx2 H6.
+  inverts IHx1.
+  inverts IHx2.
+  SCase "x1/x2 value".
+   inverts H4.
+   false.
+   SSCase "x1 ~ XLam".
+    exists (substX 0 x2 x).
+    apply EsLamApp.
+    inverts H0. auto.
+   inverts H. inverts H3.
+   inverts H. inverts H3.
+   inverts H4.
+   inverts H4.
+  SCase "x2 steps".
+   destruct H0 as [x2'].
+   exists (XApp x1 x2'). auto.
+  SCase "x1 steps".
+   destruct H  as [x1'].
+   exists (XApp x1' x2).
+   eapply (EsContext (fun xx => XApp xx x2)); auto.
+ 
  Case "XCon".
-  admit. (* finish this *)
+  inverts H0.
+  assert (Forall (fun x => whnfX x \/ (exists x', STEP x x')) xs).
+   admit. clear H. (* fine *)
+  lets D: exps_ctx_run H0.
+  inverts D.
+   left.
+    eapply Value. eauto. eauto.
+   right. 
+    destruct H as [C].
+    destruct H as [x'].
+    inverts H. inverts H2.
+    lets D2: step_XCon H1 H5.
+     destruct D2. eauto.
 
  Case "XCase".
-  subst.
-  assert (@Empty ty = Empty). auto.
-   lets D: IHTYPE H4. clear IHTYPE. clear H4.
-  inverts D.
-
-  SCase "xObj value".
-   right.
-   destruct xObj.
-    SSCase "XVar". inverts H4. inverts H6. destruct H8. false.
-    SSCase "XLam". inverts H.
-    SSCase "XApp". inverts H4. inverts H5.
+  right.
+  inverts H0.
+  specializes IHx H3.
+  inverts IHx.
+  SCase "x value".
+   destruct x.
+    SSCase "can't happen".
+     inverts H3. inverts H7.
+     inverts H3.
+     inverts H0.
+     inverts H1.
     SSCase "XCon".
-     rewrite Forall_forall in H0.
-     assert (exists tsArgs x, getAlt d alts = Some (AAlt d tsArgs x)).
-      inverts H.
-      rewrite Forall_forall in H3.
-      assert (dcs0 = dcs).
-       rewrite H2 in H11. inverts H11. auto.
-       subst.
-       apply getAlt_exists. auto.
-
-     destruct H5. destruct H5.
-     exists (substXs 0 l x0).
-     eapply EsCaseAlt.
-      inverts H4. inverts H6. auto.
+     inverts H3.
+     assert (dcs0 = dcs).
+      rewrite H8 in H12. inverts H12. auto. subst.
+     assert (exists ts x, getAlt d aa = Some (AAlt d ts x)).
+      eapply getAlt_exists.
+      rewrite Forall_forall in H10.
       eauto.
+     destruct H1 as [ts].
+     destruct H1 as [x].      
+     exists (substXs 0 l x).
+     eapply EsCaseAlt.
+      inverts H0. inverts H2. auto.
+      eauto.
+    SSCase "can't happen".
+     inverts H0. inverts H1.
+  SCase "x steps".
+   destruct H0 as [x'].
+   exists (XCase x' aa).
+   lets D: EsContext XcCase. eauto.
 
-    SSCase "XCase". 
-     inverts H4. inverts H5.   
-    
-  SCase "xObj steps".
-   right.
-   destruct H4 as [xObj'].
-   exists (XCase xObj' alts).
-    eapply (EsContext (fun xx => XCase xx alts)).
-    eauto. auto.
+ Case "XAlt".
+   auto.     
 Qed.
 
 
